proof/AdequacyLocal.v
@@ -5,45 +5,65 @@ Require Import Sem.
 Require Import ModSem.
 Require Import LinkingC.
 Require Import Skeleton.
-From Paco Require Import paco.
-Require Import sflib.
-Require Import SymbInj.
 
-Require Import SimMem.
-Require Import SimModSem.
+Require Import Pair SimSymb SimMem SimProg Ord SimModSem.
 
 Set Implicit Arguments.
 
 
 
-Inductive sim_sk (si: symbinj) (sk_src sk_tgt: Sk.t): Prop :=
-| sim_sk_intro
-    (CLOSED: symbinj_closed si sk_src sk_tgt)
-    (PRIVATE: symbinj_private si sk_src sk_tgt)
-.
+Section ADEQUACY.
 
-Inductive Forall3 X Y Z (R: X -> Y -> Z -> Prop): list X -> list Y -> list Z -> Prop :=
-| Forall3_nil: Forall3 R [] [] []
-| Forall3_cons
-    x y z
-    xs ys zs
-    (TAIL: Forall3 R xs ys zs)
-  :
-    Forall3 R (x :: xs) (y :: ys) (z :: zs)
-.
+  Context `{SS: SimSymb.class}.
+  Context `{SM: SimMem.class}.
 
-Lemma Forall3_impl
-      X Y Z
-      (xs: list X) (ys: list Y) (zs: list Z)
-      P Q
-      (IMPL: P <3= Q)
-      (FORALL: Forall3 P xs ys zs)
-  :
-    <<FORALL: Forall3 Q xs ys zs>>
-.
-Proof.
-  admit "easy".
-Qed.
+  Variable pp: ProgPair.t.
+  Hypothesis SIMPROG: sim_progpair pp.
+  Let p_src := pp.(ProgPair.src).
+  Let p_tgt := pp.(ProgPair.src).
+
+  Theorem sim_load
+        sem_src
+        (LOADSRC: sem p_src = Some sem_src)
+    :
+      exists sem_tgt, <<LOADTGT: sem p_tgt = Some sem_tgt>>
+  .
+  Proof.
+    unfold sem in *.
+    des_ifs.
+    { esplits; eauto. }
+    exfalso.
+    unfold init_sk in *.
+    admit "".
+  Qed.
+
+  Theorem adequacy_local
+          sem_src
+          (LOADSRC: sem p_src = Some sem_src)
+    :
+      exists sem_tgt, <<LOADTGT: sem p_tgt = Some sem_tgt>> /\ <<SIM: mixed_simulation sem_src sem_tgt>>
+  .
+  Proof.
+    exploit sim_load; eauto. i; des.
+    esplits; eauto.
+
+    unfold sem in *. des_ifs. rename t into init_sk_tgt. rename t0 into init_sk_src.
+    inv SIMPROG.
+    inv SIMMOD. admit "".
+    assert(Forall2 sim_modsem
+    assert(exists wfo, 
+    econs; eauto.
+    econs; eauto.
+    (* Each modsem has mixed sim *)
+
+    assert(Forall3 sim_modsem p_src p_tgt).
+    eapply Forall3_impl with (Q:= const sim_modsem) in SIMMOD.
+    
+  Qed.
+
+
+End ADEQUACY.
+
 
 Context `{Linker symbinj}.
 Context `{SM: SimMem}.
@@ -57,30 +77,6 @@ Axiom sim_skenv: list symbinj -> SkEnv.t -> SkEnv.t -> Prop.
 Axiom sim_modsem: symbinj -> ModSem.t -> ModSem.t -> Prop.
 
 
-Inductive sim_modpair (mp: ModPair.t): Prop :=
-| sim_intro
-    (SIMSK: sim_sk mp.(si) mp.(src).(Mod.sk) mp.(tgt).(Mod.sk))
-    (WF: True) (* si is well-formed according to src/tgt. So that it can link with others *)
-    (SIMMS: forall
-        skenv_src skenv_tgt
-        (SIMSKENV: respects mp.(si) skenv_src skenv_tgt)
-      ,
-        sim_modsem (mp.(si))
-                   (mp.(src).(Mod.get_modsem) skenv_src mp.(src).(Mod.data))
-                   (mp.(tgt).(Mod.get_modsem) skenv_tgt mp.(tgt).(Mod.data)))
-.
-
-
-Module ModSemPair.
-
-  Record t: Type := {
-    src: ModSem.t;
-    tgt: ModSem.t;
-    si: symbinj;
-  }
-  .
-
-End ModSemPair.
 
 Inductive sim_prog (p_src p_tgt: program): Prop :=
 | sim_prog_intro
@@ -106,57 +102,6 @@ Section ADEQUACY.
 
   Variable p_src p_tgt: program.
   Hypothesis SIMPROG: sim_prog p_src p_tgt.
-
-  Section LINK_WFO.
-
-    Variable (idx0 idx1: Type) (ord0: idx0 -> idx0 -> Prop) (ord1: idx1 -> idx1 -> Prop).
-
-    Inductive embedded A B (ordA: A -> A -> Prop) (ordB: B -> B -> Prop): Prop :=
-    | embedded_intro
-        f
-        (PRESERVING: forall
-            a0 a1
-            (ORDA: ordA a0 a1)
-          ,
-            <<ORDB: ordB (f a0) (f a1)>>)
-    .
-
-    Let idx := (idx0 + idx1)%type.
-
-    Inductive ord: idx -> idx -> Prop :=
-    | ord_introl
-        idx0a idx0b
-        (ORD0: ord0 idx0a idx0b)
-      :
-        ord (inl idx0a) (inl idx0b)
-    | ord_intror
-        idx1a idx1b
-        (ORD1: ord1 idx1a idx1b)
-      :
-        ord (inr idx1a) (inr idx1b)
-    .
-
-    Theorem link_wfo
-            
-            (WF0: well_founded ord0)
-            (WF1: well_founded ord1)
-      :
-        exists (idx: Type) (ord: idx -> idx -> Prop),
-          <<EMBED0: embedded ord0 ord>> /\ <<EMBED1: embedded ord1 ord>> /\ <<WF: well_founded ord>>
-    .
-    Proof.
-      exists idx, ord.
-      esplits; eauto.
-      - eapply embedded_intro with (f := inl). econs; eauto.
-      - eapply embedded_intro with (f := inr). econs; eauto.
-      - econs; eauto. i. inv H0.
-        + generalize dependent idx0a. pattern idx0b. eapply well_founded_ind; eauto. clear idx0b. i.
-          econs; eauto. i. inv H1.
-          eapply H0; eauto.
-        + generalize dependent idx1a. pattern idx1b. eapply well_founded_ind; eauto. clear idx1b. i.
-          econs; eauto. i. inv H1.
-          eapply H0; eauto.
-    Qed.
 
     Theorem xsim_properties_embedded
             L1 L2
