compose/Pair.v
@@ -1,0 +1,141 @@
+Require Import Events.
+Require Import Values.
+Require Import AST.
+Require Import Asmregs.
+Require Import Memory.
+Require Import Globalenvs.
+Require Import Smallstep.
+Require Import CoqlibC.
+Require Import Skeleton.
+Require Import Integers.
+Require Import ASTC.
+Require Import Maps.
+Require Import LinkingC.
+
+Require Import Syntax Mod ModSem SimSymb.
+
+Set Implicit Arguments.
+
+
+(* TODO: name? *)
+Inductive closed `{SimSymb.class} (ss: SimSymb.t) (sk_src sk_tgt: Sk.t): Prop :=
+| closed_intro
+    (WF: SimSymb.wf ss)
+    (INSRC: ss.(SimSymb.privs) <1= sk_src.(defs))
+    (INTGT: ss.(SimSymb.privs) <1= sk_tgt.(defs))
+    (PUBS: forall
+        id
+        (PUBS: ~ ss.(SimSymb.privs) id)
+      ,
+        <<EQ: PTree.get id sk_src.(prog_defmap) = PTree.get id sk_tgt.(prog_defmap)>>)
+.
+
+
+Module ModPair.
+
+  Record t: Type := {
+    src: Mod.t;
+    tgt: Mod.t;
+    SS:> SimSymb.class;
+    ss: SimSymb.t;
+    wf:= closed ss src.(Mod.sk) tgt.(Mod.sk)
+  }
+  .
+
+  Reset t. (* Need to state SS = SS in SimMem... JMEQ THINGS !!!!!!!!!!!!! *)
+
+  Record t `{SimSymb.class}: Type := {
+    src: Mod.t;
+    tgt: Mod.t;
+    ss: SimSymb.t;
+    wf:= closed ss src.(Mod.sk) tgt.(Mod.sk)
+  }
+  .
+
+  (* Change sim_modsem to be sensitive to si. *)
+  (* Only when initial memory is respecting si, it can guarantee something. *)
+  (* Q: Can we encode it inside SM? *)
+
+End ModPair.
+ 
+(* Module ModPair. *)
+
+(*   Record t: Type := { *)
+(*     src: Mod.t; *)
+(*     tgt: Mod.t; *)
+(*     si: symbinj; *)
+(*     (* TODO: unify closed & private *) *)
+(*     closed: symbinj_closed si src tgt; *)
+(*     private: symbinj_private si src tgt; *)
+(*     (* TODO: which unary/binary property it expects *) *)
+(*     (* TODO: analysis *) *)
+(*   } *)
+(*   . *)
+
+(*   (* Change sim_modsem to be sensitive to si. *) *)
+(*   (* Only when initial memory is respecting si, it can guarantee something. *) *)
+(*   (* Q: Can we encode it inside SM? *) *)
+
+(* End ModPair. *)
+
+
+
+
+
+
+
+
+
+
+
+
+
+
+
+
+
+
+
+
+
+
+
+
+
+(* Module ModSemPair. *)
+
+(*   Record t: Type := { *)
+(*     src: ModSem.t; *)
+(*     tgt: ModSem.t; *)
+(*     si: symbinj; *)
+(*     (* TODO: unify closed & private *) *)
+(*     closed: symbinj_closed si src tgt; *)
+(*     private: symbinj_private si src tgt; *)
+(*     (* TODO: which unary/binary property it expects *) *)
+(*     (* TODO: analysis *) *)
+(*   } *)
+(*   . *)
+
+(* End ModSemPair. *)
+
+
+Module ProgPair.
+Section PROGPAIR.
+Context `{SS: SimSymb.class}.
+
+  Definition t := list ModPair.t.
+
+  Definition wf (pp: t) := List.Forall ModPair.wf pp.
+
+  Definition src (pp: t): program := List.map ModPair.src pp.
+  Definition tgt (pp: t): program := List.map ModPair.tgt pp.
+
+  Definition ss_link (pp: t): option SimSymb.t := link_list (List.map ModPair.ss pp).
+  (* ############ TODO: *)
+  (* ModPair.wf mp0 /\ ModPair.wf mp1 /\ link mp0.(src) mp1.(src) = Some /\ link mp1.(tgt) mp1.(tgt) = Some *)
+  (* =================> link mp0.(ss) mp1.(ss) suceeds. *)
+  (* Move ModPair.wf into SimSymb and obligate its proof? *)
+
+End PROGPAIR.
+End ProgPair.
+
