compose/Syntax.v
@@ -1,0 +1,17 @@
+Require Import Maps.
+Require Import AST.
+Require Import Integers.
+Require Import Values.
+Require Import Memory.
+Require Import Events.
+Require Import Smallstep.
+Require Import Globalenvs.
+Require Import Asmregs.
+Require Import Linking.
+Require Import CoqlibC.
+Require Import sflib.
+
+Require Import ModSem Mod Skeleton LinkingC.
+
+Definition program := list Mod.t.
+
