proof/Ord.v
@@ -1,0 +1,58 @@
+Require Import CoqlibC.
+
+Set Implicit Arguments.
+
+
+
+Section LINK_WFO.
+
+  Variable (idx0 idx1: Type) (ord0: idx0 -> idx0 -> Prop) (ord1: idx1 -> idx1 -> Prop).
+
+  Inductive embedded A B (ordA: A -> A -> Prop) (ordB: B -> B -> Prop): Prop :=
+  | embedded_intro
+      f
+      (PRESERVING: forall
+          a0 a1
+          (ORDA: ordA a0 a1)
+        ,
+          <<ORDB: ordB (f a0) (f a1)>>)
+  .
+
+  Let idx := (idx0 + idx1)%type.
+
+  Inductive ord: idx -> idx -> Prop :=
+  | ord_introl
+      idx0a idx0b
+      (ORD0: ord0 idx0a idx0b)
+    :
+      ord (inl idx0a) (inl idx0b)
+  | ord_intror
+      idx1a idx1b
+      (ORD1: ord1 idx1a idx1b)
+    :
+      ord (inr idx1a) (inr idx1b)
+  .
+
+  Theorem link_wfo
+          
+          (WF0: well_founded ord0)
+          (WF1: well_founded ord1)
+    :
+      exists (idx: Type) (ord: idx -> idx -> Prop),
+        <<EMBED0: embedded ord0 ord>> /\ <<EMBED1: embedded ord1 ord>> /\ <<WF: well_founded ord>>
+  .
+  Proof.
+    exists idx, ord.
+    esplits; eauto.
+    - eapply embedded_intro with (f := inl). econs; eauto.
+    - eapply embedded_intro with (f := inr). econs; eauto.
+    - econs; eauto. i. inv H.
+      + generalize dependent idx0a. pattern idx0b. eapply well_founded_ind; eauto. clear idx0b. i.
+        econs; eauto. i. inv H0.
+        eapply H; eauto.
+      + generalize dependent idx1a. pattern idx1b. eapply well_founded_ind; eauto. clear idx1b. i.
+        econs; eauto. i. inv H0.
+        eapply H; eauto.
+  Qed.
+
+End LINK_WFO.
