proof/SimMod.v
@@ -1,0 +1,72 @@
+Require Import Events.
+Require Import Values.
+Require Import AST.
+Require Import Asmregs.
+Require Import Memory.
+Require Import Globalenvs.
+Require Import Smallstep.
+Require Import CoqlibC.
+Require Import Skeleton.
+Require Import ModSem.
+Require Import SimSymb.
+Require Import Integers.
+Require Import ASTC.
+Require Import Maps.
+
+Require Import Syntax Sem Mod Pair ModSem SimMem SimModSem.
+
+Set Implicit Arguments.
+
+
+
+
+
+
+Section SIM.
+
+  Context `{SS: SimSymb.class} `{SM: SimMem.class}.
+
+  Inductive sim_modpair (mp: ModPair.t): Prop :=
+  | intro_sim_modpair
+      (WF: ModPair.wf mp)
+      (SIMMS: forall
+          skenv_src skenv_tgt
+          (SIMSKENV: SimSymb.sim_skenv mp.(ModPair.ss) skenv_src skenv_tgt)
+        ,
+          sim_modsem
+            (mp.(ModPair.src).(Mod.get_modsem) skenv_src mp.(ModPair.src).(Mod.data))
+            (mp.(ModPair.tgt).(Mod.get_modsem) skenv_tgt mp.(ModPair.tgt).(Mod.data)))
+  .
+
+  Inductive sim_progpair (pp: ProgPair.t): Prop :=
+  | intro_sim_modpairs
+      (SIMMP: List.Forall sim_modpair pp)
+  .
+
+End SIM.
+
+
+
+
+
+(* Inductive sim_sk (si: symbinj) (sk_src sk_tgt: Sk.t): Prop := *)
+(* | sim_sk_intro *)
+(*     (CLOSED: symbinj_closed si sk_src sk_tgt) *)
+(*     (PRIVATE: symbinj_private si sk_src sk_tgt) *)
+(* . *)
+
+
+(*   Inductive sim_modpair (mp: ModPair.t): Prop := *)
+(* | sim_intro *)
+(*     (SIMSK: sim_sk mp.(si) mp.(src).(Mod.sk) mp.(tgt).(Mod.sk)) *)
+(*     (WF: True) (* si is well-formed according to src/tgt. So that it can link with others *) *)
+(*     (SIMMS: forall *)
+(*         skenv_src skenv_tgt *)
+(*         (SIMSKENV: respects mp.(si) skenv_src skenv_tgt) *)
+(*       , *)
+(*         sim_modsem (mp.(si)) *)
+(*                    (mp.(src).(Mod.get_modsem) skenv_src mp.(src).(Mod.data)) *)
+(*                    (mp.(tgt).(Mod.get_modsem) skenv_tgt mp.(tgt).(Mod.data))) *)
+(* . *)
+
+ 
