proof/SimProg.v
@@ -1,0 +1,115 @@
+Require Import Events.
+Require Import Values.
+Require Import AST.
+Require Import Asmregs.
+Require Import Memory.
+Require Import Globalenvs.
+Require Import Smallstep.
+Require Import CoqlibC.
+Require Import Skeleton.
+Require Import ModSem.
+Require Import SimSymb.
+Require Import Integers.
+Require Import ASTC.
+Require Import Maps.
+Require Import LinkingC.
+
+Require Import Syntax Sem Mod Pair ModSem SimMem SimModSem SimMod.
+
+Set Implicit Arguments.
+
+
+
+
+
+
+Section SIM.
+
+  Context `{SS: SimSymb.class} `{SM: SimMem.class}.
+
+  Inductive sim_progpair (pp: ProgPair.t): Prop :=
+  | intro_sim_modpairs
+      (SIMMPS: List.Forall sim_modpair pp)
+  .
+
+
+
+  Variable pp: ProgPair.t.
+  Hypothesis WF: ProgPair.wf pp.
+  Hypothesis SIMPROG: sim_progpair pp.
+  Let p_src := pp.(ProgPair.src).
+  Let p_tgt := pp.(ProgPair.tgt).
+
+  Theorem sim_load
+        sem_src
+        (LOADSRC: sem p_src = Some sem_src)
+    :
+      exists sem_tgt, <<LOADTGT: sem p_tgt = Some sem_tgt>>
+  .
+  Proof.
+    unfold sem in *.
+    des_ifs.
+    { esplits; eauto. }
+    exfalso.
+    unfold init_sk in *.
+    admit "".
+  Qed.
+
+  Variable ss_link: SimSymb.t.
+  Variable sem_src sem_tgt: semantics.
+  Variable sk_src sk_tgt: Sk.t.
+  Hypothesis CLOSED: closed ss_link sk_src sk_tgt.
+  Hypothesis LINKSRC: p_src.(init_sk) = Some sk_src.
+  Hypothesis LINKTGT: p_tgt.(init_sk) = Some sk_tgt.
+  Hypothesis LOADSRC: sem p_src = Some sem_src.
+  Hypothesis LOADTGT: sem p_tgt = Some sem_tgt.
+  Hypothesis SSLINK: pp.(ProgPair.ss_link) = Some ss_link.
+
+  Inductive sim_ge (ge_src ge_tgt: Ge.t): Prop :=
+  | sim_ge_intro
+      (SKENV: SimSymb.sim_skenv ss_link ge_src.(Ge.skenv) ge_tgt.(Ge.skenv))
+      (MSS: List.Forall2 sim_modsem ge_src.(Ge.mss) ge_tgt.(Ge.mss))
+  .
+
+  Let skenv_src := sk_src.(Sk.load_skenv).
+  Let skenv_tgt := sk_tgt.(Sk.load_skenv).
+  Variable m_src m_tgt: mem.
+  Hypothesis LOADMEMSRC: sk_src.(Sk.load_mem) = Some m_src.
+  Hypothesis LOADMEMTGT: sk_tgt.(Sk.load_mem) = Some m_tgt.
+  Let ge_src := (p_src.(load_genv) skenv_src).
+  (* TODO: I want to use "sem_src.(globalenv)" here, without unfolding it. *)
+  Let ge_tgt := (p_tgt.(load_genv) skenv_tgt).
+
+  Theorem sim_progpair_sim_ge
+    :
+      sim_ge ge_src ge_tgt
+  .
+  Proof.
+    assert(SIMSKENV: SimSymb.sim_skenv ss_link ge_src.(Ge.skenv) ge_tgt.(Ge.skenv)).
+    { exploit SimMem.load_respects_ss; eauto. i; des. ss. }
+    econs; eauto.
+    inv SIMPROG.
+    cbn.
+    clear - SIMMPS SIMSKENV SSLINK.
+    unfold ProgPair.ss_link in *.
+    assert(LINKORDER: forall
+              ss
+              (IN: List.In ss (map ModPair.ss pp))
+            ,
+              <<LO: linkorder ss ss_link>>).
+    { i. admit "link_list_linkorder". }
+    subst skenv_src skenv_tgt ge_src ge_tgt p_src p_tgt.
+    ginduction pp; ii; ss.
+    unfold flip. inv SIMMPS.
+    econs; eauto.
+    - eapply H1; eauto.
+      eapply SimSymb.sim_skenv_monotone_ss; eauto.
+      admit "link_list_linkorder".
+    - eapply IHt; eauto.
+      admit "link_list_linkorder".
+  Qed.
+
+End SIM.
+
+
+
